add better automation

IrisCore/Automation.thy
@@ -6,37 +6,91 @@ method itac = tactic all_tac
 
 method iIntro = 
   (match conclusion in "upred_holds _" \<Rightarrow> \<open>rule upred_wand_holdsI\<close>)?,((rule upred_wandI)+)?
+
+text \<open>A simple attribute to convert upred_holds predicates into entailments.\<close>
+ML \<open> val to_entailment: attribute context_parser = let 
+  fun is_upred_holds (Const(\<^const_name>\<open>Trueprop\<close>,_)$(Const(\<^const_name>\<open>upred_holds\<close>,_)$_)) = true
+    | is_upred_holds _ = false
+  fun match_upred_holds thm = is_upred_holds (Thm.concl_of thm)
+
+  fun is_wand_term (Const(\<^const_name>\<open>upred_wand\<close>,_)$_$_) = true
+    | is_wand_term _ = false
+
+  fun contains_wand thm = Thm.concl_of thm
+    |> dest_comb |> snd (* Strip Trueprop*)
+    |> strip_comb |> snd |> tl |> hd (* Strip entails*)
+    |> is_wand_term
+
+  fun contains_emp (Const(\<^const_name>\<open>upred_pure\<close>,_)$Const(\<^const_name>\<open>True\<close>,_)) = true
+    | contains_emp (f$x) = contains_emp f orelse contains_emp x
+    | contains_emp _ = false
+
+  fun remove_emp thm = if contains_emp (Thm.concl_of thm
+      |> dest_comb |> snd (* Strip Trueprop*)
+      |> strip_comb |> snd |> hd (* Strip entails*))
+    then Conv.fconv_rule (Conv.rewr_conv @{thm  eq_reflection[OF upred_sep_comm]}
+      then_conv (Conv.rewr_conv @{thm  eq_reflection[OF upred_true_sep]})
+      |> Conv.arg_conv (* Only transform the antecedent *)
+      |> Conv.fun_conv (* Go below the "\<turnstile>" *) 
+      |> HOLogic.Trueprop_conv
+      |> Conv.concl_conv ~1)
+      thm
+    else thm
+
+  fun to_entail thm = (if match_upred_holds thm 
+    then Conv.fconv_rule (Conv.rewr_conv @{thm eq_reflection[OF upred_holds_entails]}
+      |> HOLogic.Trueprop_conv
+      |> Conv.concl_conv ~1)
+      thm
+    else thm)
+
+  fun move_wands thm = (if contains_wand thm then (@{thm upred_wandE} OF [thm]) |> remove_emp |> move_wands
+    else thm)
+  in
+    (fn whatevs => ((fn (ctxt, thm) => let val thm' = try (move_wands o to_entail) thm in
+    (SOME ctxt, thm')end), whatevs)) end
+
+\<close>
+attribute_setup to_entailment = \<open>to_entailment\<close>
+
+method entails_substL uses rule = 
+  match rule[uncurry] in "_ = _" \<Rightarrow> \<open>rule upred_entails_trans[OF upred_entails_eq[OF rule]]\<close>
+  \<bar> "_ \<Longrightarrow> (_=_)" \<Rightarrow> \<open>rule upred_entails_trans[OF upred_entails_eq[OF rule]]\<close>
+  \<bar> "_\<turnstile>_" \<Rightarrow> \<open>rule rule
+    | rule upred_entails_substE[OF rule, unfolded upred_sep_assoc_eq]
+    | rule upred_entails_trans[OF rule] | rule upred_entails_substE'[OF rule, unfolded upred_conj_assoc]\<close>
+  \<bar> "_ \<Longrightarrow> (_ \<turnstile> _)" \<Rightarrow> \<open>rule rule
+    | rule upred_entails_substE[OF rule, unfolded upred_sep_assoc_eq]
+    | rule upred_entails_trans[OF rule] | rule upred_entails_substE'[OF rule, unfolded upred_conj_assoc]\<close>
+  \<bar> R[curry]: "upred_holds _" \<Rightarrow> \<open>entails_substL rule: R[to_entailment]\<close>
+  \<bar> R[curry]: "_ \<Longrightarrow> upred_holds _" \<Rightarrow> \<open>entails_substL rule: R[to_entailment]\<close>
   
-method entails_substL uses rule rule_eq = 
-  (match rule_eq in "_ = _" \<Rightarrow> \<open>rule upred_entails_trans[OF upred_entails_eq[OF rule_eq]]\<close>)
-| (match rule in "_" \<Rightarrow> \<open>rule upred_entails_substE[OF rule, unfolded upred_sep_assoc_eq]\<close>)
-| (match rule in "_" \<Rightarrow> \<open>rule upred_entails_trans[OF rule]\<close>)
-| (match rule in "_" \<Rightarrow> \<open>rule upred_entails_substE'[OF rule, unfolded upred_conj_assoc]\<close>)
-
-method entails_substR uses rule rule_eq = 
-  (match rule_eq in "_ = _" \<Rightarrow> \<open>rule upred_entails_trans[OF _ upred_entails_eq[OF rule_eq]]\<close>)
-| (match rule in "_" \<Rightarrow> \<open>rule upred_entails_substI[OF rule, unfolded upred_sep_assoc_eq]\<close>)
-| (match rule in "_" \<Rightarrow> \<open>rule upred_entails_trans[OF _ rule]\<close>)
-
+method entails_substR uses rule = 
+  match rule[uncurry] in "_ = _" \<Rightarrow> \<open>rule upred_entails_trans[OF _ upred_entails_eq[OF rule]]\<close>
+  \<bar> "_ \<Longrightarrow> (_=_)" \<Rightarrow> \<open>rule upred_entails_trans[OF _ upred_entails_eq[OF rule]]\<close>
+  \<bar> "_\<turnstile>_" \<Rightarrow> \<open>rule upred_entails_substI[OF rule, unfolded upred_sep_assoc_eq]
+    | rule upred_entails_trans[OF _ rule]\<close>
+  \<bar> "_ \<Longrightarrow> (_ \<turnstile> _)" \<Rightarrow> \<open>rule upred_entails_substI[OF rule, unfolded upred_sep_assoc_eq]
+    | rule upred_entails_trans[OF _ rule]\<close>
+  \<bar> "upred_holds (P-\<^emph>Q)" for P Q \<Rightarrow> \<open>entails_substR rule: upred_wand_holdsE[OF rule]\<close>
+  \<bar> "_ \<Longrightarrow> upred_holds (P-\<^emph>Q)" for P Q \<Rightarrow> \<open>entails_substR rule: upred_wand_holdsE[OF rule]\<close>
+  \<bar> R[curry]: "upred_holds _" \<Rightarrow> \<open>entails_substR rule: R[to_entailment]\<close>
+  \<bar> R[curry]: "_ \<Longrightarrow> upred_holds _" \<Rightarrow> \<open>entails_substR rule: R[to_entailment]\<close>
+  
 method dupl_pers = (entails_substL rule: upred_entail_eqR[OF persistent_dupl], (pers_solver; fail))?
-
+                                               
 method subst_pers_keepL uses rule =
   (entails_substL rule: persistent_keep[OF _ rule], (pers_solver; fail))
 | entails_substL rule: rule
 
-method find_pat_sep for pat trm :: "'a::ucamera upred_f" = 
-  match (trm) in "pat" \<Rightarrow> itac
-  \<bar> "_\<^emph>pat" \<Rightarrow> itac
-  \<bar> "pat\<^emph>_" \<Rightarrow> itac
-  \<bar> "rest\<^emph>_" for rest :: "'a upred_f" \<Rightarrow> \<open>find_pat_sep pat rest\<close>   
-
+text \<open>Unchecked move methods, might not terminate if pattern is not found.\<close>
 method move_sepL for pat :: "'a::ucamera upred_f" =
-  match conclusion in \<open>hyps \<turnstile> goal\<close> for hyps goal :: "'a upred_f" \<Rightarrow>
-    \<open> find_pat_sep pat hyps; match (hyps) in "pat" \<Rightarrow> itac
+  match conclusion in \<open>hyps \<turnstile> _\<close> for hyps :: "'a upred_f" \<Rightarrow>
+    \<open> match (hyps) in "pat" \<Rightarrow> itac
       \<bar> "_\<^emph>pat" \<Rightarrow> itac
       \<bar> "pat\<^emph>_" \<Rightarrow> \<open>subst upred_sep_comm\<close>
       \<bar> "_\<^emph>pat\<^emph>_" \<Rightarrow> \<open>entails_substL rule: upred_sep_comm2R\<close>
-      \<bar> "pat\<^emph>_\<^emph>_" \<Rightarrow> \<open>entails_substL rule_eq: upred_sep_comm2L; move_sepL pat\<close>
+      \<bar> "pat\<^emph>_\<^emph>_" \<Rightarrow> \<open>entails_substL rule: upred_sep_comm2L; move_sepL pat\<close>
       \<bar> "_\<^emph>pat\<^emph>_\<^emph>_" \<Rightarrow> \<open>entails_substL rule: upred_sep_comm3M; move_sepL pat\<close>
       \<bar> "pat\<^emph>_\<^emph>_\<^emph>_" \<Rightarrow> \<open>entails_substL rule: upred_sep_comm3L; move_sepL pat\<close>
       \<bar> "_\<^emph>pat\<^emph>_\<^emph>_\<^emph>_" \<Rightarrow> \<open>entails_substL rule: upred_sep_comm4_2; move_sepL pat\<close>
@@ -53,12 +107,12 @@ method move_sepL for pat :: "'a::ucamera upred_f" =
     \<close>
 
 method move_sepR for pat :: "'a::ucamera upred_f" =
-  match conclusion in \<open>hyps \<turnstile> goal\<close> for hyps goal :: "'a upred_f" \<Rightarrow>
-    \<open> find_pat_sep pat goal; match (goal) in "pat" \<Rightarrow> itac
+  match conclusion in \<open>_ \<turnstile> goal\<close> for goal :: "'a upred_f" \<Rightarrow>
+    \<open> match (goal) in "pat" \<Rightarrow> itac
       \<bar> "_\<^emph>pat" \<Rightarrow> itac
-      \<bar> "pat\<^emph>_" \<Rightarrow> \<open>entails_substR rule_eq: upred_sep_comm\<close>
+      \<bar> "pat\<^emph>_" \<Rightarrow> \<open>entails_substR rule: upred_sep_comm\<close>
       \<bar> "_\<^emph>pat\<^emph>_" \<Rightarrow> \<open>entails_substR rule: upred_sep_comm2R\<close>
-      \<bar> "pat\<^emph>_\<^emph>_" \<Rightarrow> \<open>entails_substR rule_eq: upred_sep_comm2L; move_sepR pat\<close>
+      \<bar> "pat\<^emph>_\<^emph>_" \<Rightarrow> \<open>entails_substR rule: upred_sep_comm2L; move_sepR pat\<close>
       \<bar> "_\<^emph>pat\<^emph>_\<^emph>_" \<Rightarrow> \<open>entails_substR rule: upred_sep_comm3M; move_sepR pat\<close>
       \<bar> "pat\<^emph>_\<^emph>_\<^emph>_" \<Rightarrow> \<open>entails_substR rule: upred_sep_comm3L; move_sepR pat\<close>
       \<bar> "_\<^emph>pat\<^emph>_\<^emph>_\<^emph>_" \<Rightarrow> \<open>entails_substR rule: upred_sep_comm4_2; move_sepR pat\<close>
@@ -85,45 +139,128 @@ method move_sep_all for left :: bool and trm :: "'a::ucamera upred_f" =
 method move_sep_both for trm :: "'a::ucamera upred_f" =
   move_sepL trm, move_sepR trm
 
+text \<open>Checked move methods, will terminate.\<close>
+method find_pat_sep for pat trm :: "'a::ucamera upred_f" = 
+  match (trm) in "pat" \<Rightarrow> itac
+  \<bar> "_\<^emph>pat" \<Rightarrow> itac
+  \<bar> "pat\<^emph>_" \<Rightarrow> itac
+  \<bar> "rest\<^emph>_" for rest :: "'a upred_f" \<Rightarrow> \<open>find_pat_sep pat rest\<close>   
+
+method check_moveL for pat :: "'a::ucamera upred_f" =
+  match conclusion in \<open>hyps \<turnstile> _\<close> for hyps :: "'a upred_f" \<Rightarrow>
+    \<open> find_pat_sep pat hyps; move_sepL pat\<close>
+    
+method check_moveR for pat :: "'a::ucamera upred_f" =
+  match conclusion in \<open>_ \<turnstile> goal\<close> for goal :: "'a upred_f" \<Rightarrow>
+    \<open> find_pat_sep pat goal; move_sepR pat\<close>
+    
+method check_move for left :: bool and pat :: "'a::ucamera upred_f" = 
+  match (left) in True \<Rightarrow> \<open>check_moveL pat\<close>
+  \<bar> False \<Rightarrow> \<open>check_moveR pat\<close>  
+
+method check_move_all for left :: bool and trm :: "'a::ucamera upred_f" =
+  match (trm) in "rest\<^emph>head" for rest head :: "'a upred_f" \<Rightarrow> \<open>check_move_all left rest; check_move left head\<close>
+  \<bar> "P" for P :: "'a upred_f" \<Rightarrow> \<open>check_move left P\<close>
+
+method check_move_both for trm :: "'a::ucamera upred_f" =
+  check_moveL trm, check_moveR trm
+
+method check_move_dupl_all for left acc_pure :: bool and trm :: "'a::ucamera upred_f" =
+  match (trm) in "rest\<^emph>\<upharpoonleft>_" for rest :: "'a upred_f" \<Rightarrow> \<open>match (acc_pure) in True \<Rightarrow> itac 
+    \<bar> False \<Rightarrow> \<open>check_move left head, dupl_pers, check_move_dupl_all left acc_pure rest\<close>\<close>
+  \<bar> "rest\<^emph>head" for rest head :: "'a upred_f" \<Rightarrow>
+    \<open>check_move left head, dupl_pers, check_move_dupl_all left acc_pure rest\<close>
+  \<bar> "P" for P :: "'a upred_f" \<Rightarrow> \<open>check_move left P, dupl_pers\<close>
+
+text \<open>Moves all hypotheses while duplicating all persistent, then moves again but unchecked to get 
+  correct order of hypotheses. Then applies given rule.\<close>
 method iApply uses rule =
-  match rule in "hyps \<turnstile> goal" for hyps goal \<Rightarrow> \<open>move_sep_all True hyps, subst_pers_keepL rule: rule\<close>
-  \<bar> "_ \<Longrightarrow> hyps \<turnstile> goal" for hyps goal \<Rightarrow> \<open>move_sep_all True hyps, subst_pers_keepL rule: rule\<close>
+  match rule[uncurry] in "hyps \<turnstile> _" for hyps \<Rightarrow> \<open>check_move_dupl_all True True hyps, move_sep_all True hyps, 
+    subst_pers_keepL rule: rule\<close>
+  \<bar> "_ \<Longrightarrow> hyps \<turnstile> _" for hyps \<Rightarrow> \<open>check_move_dupl_all True True hyps, move_sep_all True hyps,
+    subst_pers_keepL rule: rule\<close>
+  \<bar> R[curry]: "upred_holds _" \<Rightarrow> \<open>iApply rule: R[to_entailment]\<close>
+  \<bar> R[curry]: "_ \<Longrightarrow> upred_holds _" \<Rightarrow> \<open>iApply rule: R[to_entailment]\<close>
+
+text \<open>Due to the limitations of subgoal focusing, this can only take concrete terms to
+  separate into the left side and not a pattern.\<close>
+method split_pat for trm :: "'a::ucamera upred_f" =
+  ((match conclusion in "can_be_split (_\<^emph>_) _ _" \<Rightarrow> itac),
+  (((match conclusion in "can_be_split (_\<^emph>head) _ _" for head :: "'a upred_f" \<Rightarrow> 
+    \<open>find_pat_sep head trm\<close>), rule can_be_split_sepL)
+    | rule can_be_split_sepR), split_pat trm)
+| ((match conclusion in "can_be_split (_\<or>\<^sub>u_) _ _" \<Rightarrow> itac),rule can_be_split_disj;
+  (rule can_be_split_rev, split_pat trm))
+| ((match conclusion in "can_be_split _ _ _" \<Rightarrow> itac),
+  (((match conclusion in "can_be_split (_\<^emph>head) _ _" for head :: "'a upred_f" \<Rightarrow> 
+    \<open>find_pat_sep head pat\<close>), rule can_be_split_baseL)
+    | rule can_be_split_baseR)) 
+
+text \<open>Separates the top terms (the same number as the patterns) to the left and the rest to the right.
+  If it should separate the terms in the pattern, they first need to be moved to the top level.\<close>
+method ord_split_pat for pat :: "'a::ucamera upred_f" =
+  (match conclusion in "can_be_split (_\<^emph>_) _ _" \<Rightarrow> itac),
+  match (pat) in "rest\<^emph>_" for rest :: "'a upred_f" \<Rightarrow> \<open>rule can_be_split_sepL, ord_split_pat rest\<close>
+  \<bar> "_" \<Rightarrow> \<open>(rule can_be_split_rev, rule can_be_split_refl) | rule can_be_split_baseL\<close>
+| (match conclusion in "can_be_split (_\<or>\<^sub>u_) _ _" \<Rightarrow> itac),rule can_be_split_disj; 
+  ord_split_pat pat
+
+text \<open>Uses the rule to do a step and separates arguments based on the pat.\<close>
+method iApply_step for pat :: "'a::ucamera upred_f" uses rule =
+  check_move_all True pat, rule split_trans'[OF rule], ord_split_pat pat
+
+text \<open>Does a transitive step with the given step term and separates arguments based on pat.\<close>
+method iApply_step2 for step pat :: "'a::ucamera upred_f" =
+  check_move_all True pat, rule split_trans[where ?Q = step], ord_split_pat pat  
+  
+method remove_emp = 
+  (simp only: upred_sep_assoc_eq)?;
+  (check_moveL upred_emp; simp only: upred_true_sep; remove_emp)?;
+  (check_moveR upred_emp; simp only: upred_true_sep upred_emp_entailed; remove_emp)?
   
 method iExistsL =
-  (move_sepL "upred_exists ?P", (rule pull_exists_antecedentR)+; rule upred_existsE';
+  (check_moveL "upred_exists ?P", (rule pull_exists_antecedentR)+; rule upred_existsE';
     (simp only: upred_sep_assoc_eq)?)
+
 method iExistsR for inst =
-  (move_sepR "upred_exists ?P"; (unfold pull_exists_eq pull_exists_eq')?; 
+  (check_moveR "upred_exists ?P"; (unfold pull_exists_eq pull_exists_eq')?; 
     rule upred_existsI[of _ _ inst]; (simp only: upred_sep_assoc_eq)?)
 
-method iPureL for dupl =
-  (move_sepL "upred_pure ?b", match (dupl) in True \<Rightarrow> dupl_pers \<bar> False \<Rightarrow> itac, rule upred_pure_impl)
+method iPureL =
+  (check_moveL "upred_pure ?b", rule upred_pure_impl)
 
 method iPureR = 
-  (move_sepR "upred_pure ?b", (rule upred_pureI' | rule upred_pureI))
+  (check_moveR "upred_pure ?b", rule upred_pureI' upred_pureI; (simp only: simp_thms(6))?; remove_emp)
   
-method find_applicable_wand for whole trm :: "'a::ucamera upred_f" =
+method find_applicable_wand for trm :: "'a::ucamera upred_f" =
   match (trm) in "P-\<^emph>Q" for P Q :: "'a upred_f" \<Rightarrow>
-    \<open>find_pat_sep P whole; move_sepL P; dupl_pers; move_sepL "P-\<^emph>Q"\<close>
-  \<bar> "_\<^emph>(P-\<^emph>Q)" for P Q :: "'a upred_f" \<Rightarrow>
-    \<open>find_pat_sep P whole; move_sepL P; dupl_pers; move_sepL "P-\<^emph>Q"\<close>
-  \<bar> "rest\<^emph>_" for rest :: "'a upred_f" \<Rightarrow> \<open>find_applicable_wand whole rest\<close>
+    \<open>check_moveL P, dupl_pers, move_sepL "P-\<^emph>Q"\<close>
+  \<bar> "rest\<^emph>(P-\<^emph>Q)" for P Q rest :: "'a upred_f" \<Rightarrow>
+    \<open>(check_moveL P, dupl_pers, move_sepL "P-\<^emph>Q") | find_applicable_wand rest\<close>
+  \<bar> "rest\<^emph>_" for rest :: "'a upred_f" \<Rightarrow> \<open>find_applicable_wand rest\<close>
 
 method iApply_wand =
-  match conclusion in \<open>hyps \<turnstile> goal\<close> for hyps goal \<Rightarrow>
-    \<open>find_applicable_wand hyps hyps; subst_pers_keepL rule: upred_wand_apply\<close>
+  match conclusion in \<open>hyps \<turnstile> _\<close> for hyps \<Rightarrow>
+    \<open>find_applicable_wand hyps, subst_pers_keepL rule: upred_wand_apply, remove_emp\<close>
 
+text \<open>Tries to remove the head goal term by either framing or reasoning with iPure and assumptions.\<close>
 method iFrame_single = 
-  match conclusion in \<open>hyps \<turnstile> goal\<close> for hyps goal :: "'a::ucamera upred_f" \<Rightarrow>
-    \<open> match (goal) in "_\<^emph>P" for P \<Rightarrow> \<open>move_sepL P; dupl_pers; rule upred_frame\<close> 
+  remove_emp, match conclusion in \<open>_ \<turnstile> goal\<close> for goal :: "'a::ucamera upred_f" \<Rightarrow>
+    \<open> match (goal) in "_\<^emph>P" for P \<Rightarrow> 
+        \<open> (check_moveL P; dupl_pers; rule upred_frame upred_emp_left)
+        | (iPureR; assumption)\<close>
       \<bar> P for P :: "'a upred_f" \<Rightarrow> 
-      \<open>move_sepL P; rule upred_entails_refl | rule upred_weakeningL | rule upred_weakeningR\<close> \<close>
+        \<open>(move_sepL P; (rule upred_entails_refl | rule upred_weakeningR)) | (iPureR; assumption)\<close> \<close>
 
-method remove_emp = 
-  match conclusion in \<open>hyps \<turnstile> goal\<close> for hyps goal :: "'a::ucamera upred_f" \<Rightarrow>
-    \<open>(find_pat_sep upred_emp hyps; move_sepL upred_emp; simp only: upred_true_sep; remove_emp)?;
-     (find_pat_sep upred_emp goal; move_sepR upred_emp; simp only: upred_true_sep; remove_emp)?\<close>
-  
+method later_elim =
+  check_moveL "\<triangleright> ?P", 
+  (rule elim_modal_entails'[OF elim_modal_timeless']
+  | rule elim_modal_entails[OF elim_modal_timeless']),
+  (timeless_solver;fail)+, (iez_solver; fail)+
+
+method iMod_raw methods later fupd uses rule =
+  iApply rule: rule, (prefer_last, (later | fupd)+, defer_tac)?; remove_emp
+
 lemma test_lemma: "S \<^emph> (\<box>P) \<^emph> Q \<^emph> ((\<box>P)-\<^emph>\<box>R) \<^emph> (\<triangleright>R) -\<^emph> (\<box>R) \<^emph> (\<triangleright>R) \<^emph> Q"
 apply iIntro
 apply iApply_wand
